AczelSetTheory/Algebra.lean
@@ -18,3 +18,4 @@ import AczelSetTheory.Algebra.FirstIsomorphism
 import AczelSetTheory.Algebra.SecondIsomorphism
 import AczelSetTheory.Algebra.ThirdIsomorphism
 import AczelSetTheory.Algebra.CorrespondenceTheorem
+import AczelSetTheory.Algebra.Zassenhaus
